adapting to Isabelle/a095acd4cfbf

Bachmair_Ganzinger/Ground_Resolution_Model.thy
@@ -44,15 +44,15 @@ function
   production :: "'a clause \<Rightarrow> 'a interp"
 where
   "production C =
-   {A. C \<in> N \<and> C \<noteq> {#} \<and> Max (set_mset C) = Pos A \<and> \<not> (\<Union>D \<in> {D. D #\<subset># C}. production D) \<Turnstile> C \<and>
+   {A. C \<in> N \<and> C \<noteq> {#} \<and> Max (set_mset C) = Pos A \<and> \<not> (\<Union>D \<in> {D. D < C}. production D) \<Turnstile> C \<and>
       S C = {#}}"
   by auto
-  termination by (relation "{(D, C). D #\<subset># C}") (auto simp: wf_less_multiset)
+  termination by (relation "{(D, C). D < C}") (auto simp: wf_less_multiset)
 
 declare production.simps[simp del]
 
 definition interp :: "'a clause \<Rightarrow> 'a interp" where
-  "interp C = (\<Union>D \<in> {D. D #\<subset># C}. production D)"
+  "interp C = (\<Union>D \<in> {D. D < C}. production D)"
 
 lemma production_unfold:
   "production C = {A. C \<in> N \<and> C \<noteq> {#} \<and> Max (set_mset C) = Pos A \<and> \<not> interp C \<Turnstile> C \<and> S C = {#}}"
@@ -74,8 +74,8 @@ definition Interp :: "'a clause \<Rightarrow> 'a interp" where
 lemma interp_subseteq_Interp[simp]: "interp C \<subseteq> Interp C"
   unfolding Interp_def by simp
 
-lemma Interp_as_UNION: "Interp C = (\<Union>D \<in> {D. D #\<subseteq># C}. production D)"
-  unfolding Interp_def interp_def le_multiset_def by fast
+lemma Interp_as_UNION: "Interp C = (\<Union>D \<in> {D. D \<le> C}. production D)"
+  unfolding Interp_def interp_def less_eq_multiset_def by fast
 
 lemma productive_not_empty: "productive C \<Longrightarrow> C \<noteq> {#}"
   unfolding production_unfold by simp
@@ -106,37 +106,37 @@ lemma produces_imp_atms_leq: "produces C A \<Longrightarrow> B \<in> atms_of C \
 lemma produces_imp_neg_notin_lits: "produces C A \<Longrightarrow> \<not> Neg A \<in># C"
   by (auto intro!: pos_Max_imp_neg_notin dest: producesD simp del: not_gr_zero)
 
-lemma less_eq_imp_interp_subseteq_interp: "C #\<subseteq># D \<Longrightarrow> interp C \<subseteq> interp D"
-  unfolding interp_def by auto (metis multiset_order.order.strict_trans2)
+lemma less_eq_imp_interp_subseteq_interp: "C \<le> D \<Longrightarrow> interp C \<subseteq> interp D"
+  unfolding interp_def by auto (metis order.strict_trans2)
 
-lemma less_eq_imp_interp_subseteq_Interp: "C #\<subseteq># D \<Longrightarrow> interp C \<subseteq> Interp D"
+lemma less_eq_imp_interp_subseteq_Interp: "C \<le> D \<Longrightarrow> interp C \<subseteq> Interp D"
   unfolding Interp_def using less_eq_imp_interp_subseteq_interp by blast
 
-lemma less_imp_production_subseteq_interp: "C #\<subset># D \<Longrightarrow> production C \<subseteq> interp D"
+lemma less_imp_production_subseteq_interp: "C < D \<Longrightarrow> production C \<subseteq> interp D"
   unfolding interp_def by fast
 
-lemma less_eq_imp_production_subseteq_Interp: "C #\<subseteq># D \<Longrightarrow> production C \<subseteq> Interp D"
+lemma less_eq_imp_production_subseteq_Interp: "C \<le> D \<Longrightarrow> production C \<subseteq> Interp D"
   unfolding Interp_def using less_imp_production_subseteq_interp
-  by (metis multiset_order.le_imp_less_or_eq le_supI1 sup_ge2)
+  by (metis le_imp_less_or_eq le_supI1 sup_ge2)
 
-lemma less_imp_Interp_subseteq_interp: "C #\<subset># D \<Longrightarrow> Interp C \<subseteq> interp D"
+lemma less_imp_Interp_subseteq_interp: "C < D \<Longrightarrow> Interp C \<subseteq> interp D"
   unfolding Interp_def
   by (auto simp: less_eq_imp_interp_subseteq_interp less_imp_production_subseteq_interp)
 
-lemma less_eq_imp_Interp_subseteq_Interp: "C #\<subseteq># D \<Longrightarrow> Interp C \<subseteq> Interp D"
+lemma less_eq_imp_Interp_subseteq_Interp: "C \<le> D \<Longrightarrow> Interp C \<subseteq> Interp D"
   using less_imp_Interp_subseteq_interp
-  unfolding Interp_def by (metis multiset_order.le_imp_less_or_eq le_supI2 subset_refl sup_commute)
+  unfolding Interp_def by (metis le_imp_less_or_eq le_supI2 subset_refl sup_commute)
 
-lemma false_Interp_to_true_interp_imp_less_multiset: "A \<notin> Interp C \<Longrightarrow> A \<in> interp D \<Longrightarrow> C #\<subset># D"
+lemma false_Interp_to_true_interp_imp_less_multiset: "A \<notin> Interp C \<Longrightarrow> A \<in> interp D \<Longrightarrow> C < D"
   using less_eq_imp_interp_subseteq_Interp multiset_linorder.not_less by blast
 
-lemma false_interp_to_true_interp_imp_less_multiset: "A \<notin> interp C \<Longrightarrow> A \<in> interp D \<Longrightarrow> C #\<subset># D"
+lemma false_interp_to_true_interp_imp_less_multiset: "A \<notin> interp C \<Longrightarrow> A \<in> interp D \<Longrightarrow> C < D"
   using less_eq_imp_interp_subseteq_interp multiset_linorder.not_less by blast
 
-lemma false_Interp_to_true_Interp_imp_less_multiset: "A \<notin> Interp C \<Longrightarrow> A \<in> Interp D \<Longrightarrow> C #\<subset># D"
+lemma false_Interp_to_true_Interp_imp_less_multiset: "A \<notin> Interp C \<Longrightarrow> A \<in> Interp D \<Longrightarrow> C < D"
   using less_eq_imp_Interp_subseteq_Interp multiset_linorder.not_less by blast
 
-lemma false_interp_to_true_Interp_imp_le_multiset: "A \<notin> interp C \<Longrightarrow> A \<in> Interp D \<Longrightarrow> C #\<subseteq># D"
+lemma false_interp_to_true_Interp_imp_le_multiset: "A \<notin> interp C \<Longrightarrow> A \<in> Interp D \<Longrightarrow> C \<le> D"
   using less_imp_Interp_subseteq_interp multiset_linorder.not_less by blast
 
 definition INTERP :: "'a interp" where
@@ -157,15 +157,15 @@ lemma produces_imp_in_interp:
 proof -
   from d have "Max (set_mset D) = Pos A"
     using production_unfold by blast
-  hence "D #\<subset># {#Neg A#}"
+  hence "D < {#Neg A#}"
     by (auto intro: Max_pos_neg_less_multiset)
-  moreover have "{#Neg A#} #\<subseteq># C"
-    by (rule less_eq_imp_le_multiset) (rule mset_subset_eq_single[OF a_in_c])
+  moreover have "{#Neg A#} \<le> C"
+    by (rule  subset_eq_imp_le_multiset) (rule mset_subset_eq_single[OF a_in_c])
   ultimately show ?thesis
     using d by (blast dest: less_eq_imp_interp_subseteq_interp less_imp_production_subseteq_interp)
 qed
 
-lemma neg_notin_Interp_not_produce: "Neg A \<in># C \<Longrightarrow> A \<notin> Interp D \<Longrightarrow> C #\<subseteq># D \<Longrightarrow> \<not> produces D'' A"
+lemma neg_notin_Interp_not_produce: "Neg A \<in># C \<Longrightarrow> A \<notin> Interp D \<Longrightarrow> C \<le> D \<Longrightarrow> \<not> produces D'' A"
   by (auto dest: produces_imp_in_interp less_eq_imp_interp_subseteq_Interp)
 
 lemma in_production_imp_produces: "A \<in> production C \<Longrightarrow> produces C A"
@@ -187,8 +187,8 @@ If $D = D'$ and $D$ is productive, $I^D \subseteq I_{D'}$ does not hold.
 
 lemma true_Interp_imp_general:
   assumes
-    c_le_d: "C #\<subseteq># D" and
-    d_lt_d': "D #\<subset># D'" and
+    c_le_d: "C \<le> D" and
+    d_lt_d': "D < D'" and
     c_at_d: "Interp D \<Turnstile> C" and
     subs: "interp D' \<subseteq> (\<Union>C \<in> CC. production C)"
   shows "(\<Union>C \<in> CC. production C) \<Turnstile> C"
@@ -210,21 +210,21 @@ next
     using a_in_c subs not_produces_imp_notin_production by auto
 qed
 
-lemma true_Interp_imp_interp: "C #\<subseteq># D \<Longrightarrow> D #\<subset># D' \<Longrightarrow> Interp D \<Turnstile> C \<Longrightarrow> interp D' \<Turnstile> C"
+lemma true_Interp_imp_interp: "C \<le> D \<Longrightarrow> D < D' \<Longrightarrow> Interp D \<Turnstile> C \<Longrightarrow> interp D' \<Turnstile> C"
   using interp_def true_Interp_imp_general by simp
 
-lemma true_Interp_imp_Interp: "C #\<subseteq># D \<Longrightarrow> D #\<subset># D' \<Longrightarrow> Interp D \<Turnstile> C \<Longrightarrow> Interp D' \<Turnstile> C"
+lemma true_Interp_imp_Interp: "C \<le> D \<Longrightarrow> D < D' \<Longrightarrow> Interp D \<Turnstile> C \<Longrightarrow> Interp D' \<Turnstile> C"
   using Interp_as_UNION interp_subseteq_Interp true_Interp_imp_general by simp
 
-lemma true_Interp_imp_INTERP: "C #\<subseteq># D \<Longrightarrow> Interp D \<Turnstile> C \<Longrightarrow> INTERP \<Turnstile> C"
+lemma true_Interp_imp_INTERP: "C \<le> D \<Longrightarrow> Interp D \<Turnstile> C \<Longrightarrow> INTERP \<Turnstile> C"
   using INTERP_def interp_subseteq_INTERP
-    true_Interp_imp_general[OF _ less_multiset_right_total]
+    true_Interp_imp_general[OF _ le_multiset_right_total]
   by simp
 
 lemma true_interp_imp_general:
   assumes
-    c_le_d: "C #\<subseteq># D" and
-    d_lt_d': "D #\<subset># D'" and
+    c_le_d: "C \<le> D" and
+    d_lt_d': "D < D'" and
     c_at_d: "interp D \<Turnstile> C" and
     subs: "interp D' \<subseteq> (\<Union>C \<in> CC. production C)"
   shows "(\<Union>C \<in> CC. production C) \<Turnstile> C"
@@ -233,7 +233,7 @@ proof (cases "\<exists>A. Pos A \<in># C \<and> A \<in> interp D")
   then obtain A where a_in_c: "Pos A \<in># C" and a_at_d: "A \<in> interp D"
     by blast
   from a_at_d have "A \<in> interp D'"
-    using d_lt_d' less_eq_imp_interp_subseteq_interp[OF multiset_order.less_imp_le] by blast
+    using d_lt_d' less_eq_imp_interp_subseteq_interp[OF less_imp_le] by blast
   thus ?thesis
     using subs a_in_c by (blast dest: contra_subsetD)
 next
@@ -246,15 +246,15 @@ next
     using a_in_c subs not_produces_imp_notin_production by auto
 qed
 
-lemma true_interp_imp_interp: "C #\<subseteq># D \<Longrightarrow> D #\<subset># D' \<Longrightarrow> interp D \<Turnstile> C \<Longrightarrow> interp D' \<Turnstile> C"
+lemma true_interp_imp_interp: "C \<le> D \<Longrightarrow> D < D' \<Longrightarrow> interp D \<Turnstile> C \<Longrightarrow> interp D' \<Turnstile> C"
   using interp_def true_interp_imp_general by simp
 
-lemma true_interp_imp_Interp: "C #\<subseteq># D \<Longrightarrow> D #\<subset># D' \<Longrightarrow> interp D \<Turnstile> C \<Longrightarrow> Interp D' \<Turnstile> C"
+lemma true_interp_imp_Interp: "C \<le> D \<Longrightarrow> D < D' \<Longrightarrow> interp D \<Turnstile> C \<Longrightarrow> Interp D' \<Turnstile> C"
   using Interp_as_UNION interp_subseteq_Interp[of D'] true_interp_imp_general by simp
 
-lemma true_interp_imp_INTERP: "C #\<subseteq># D \<Longrightarrow> interp D \<Turnstile> C \<Longrightarrow> INTERP \<Turnstile> C"
+lemma true_interp_imp_INTERP: "C \<le> D \<Longrightarrow> interp D \<Turnstile> C \<Longrightarrow> INTERP \<Turnstile> C"
   using INTERP_def interp_subseteq_INTERP
-    true_interp_imp_general[OF _ less_multiset_right_total]
+    true_interp_imp_general[OF _ le_multiset_right_total]
   by simp
 
 lemma productive_imp_false_interp: "productive C \<Longrightarrow> \<not> interp C \<Turnstile> C"
@@ -326,10 +326,10 @@ qed
 
 lemma false_Interp_imp_general:
   assumes
-    d'_le_d: "D' #\<subseteq># D" and
+    d'_le_d: "D' \<le> D" and
     in_n_or_max_gt: "D' \<in> N \<and> S D' = {#} \<or> Max (atms_of D') < Max (atms_of D)" and
     d'_at_d: "\<not> Interp D \<Turnstile> D'" and
-    d_lt_c: "D #\<subset># C" and
+    d_lt_c: "D < C" and
     subs: "interp C \<subseteq> (\<Union>C \<in> CC. production C)"
   shows "\<not> (\<Union>C \<in> CC. production C) \<Turnstile> D'"
 proof -
@@ -344,11 +344,11 @@ proof -
       by (fast intro!: in_production_imp_produces)
     have max_c': "Max (atms_of C') = A"
       using prod_c' productive_imp_produces_Max_atom by force
-    have leq_dc': "D #\<subseteq># C'"
+    have leq_dc': "D \<le> C'"
       using a_at_d d'_at_d prod_c'
       by (auto simp: Interp_def intro: false_interp_to_true_Interp_imp_le_multiset)
-    hence "D' #\<subseteq># C'"
-      using d'_le_d multiset_order.le_trans by blast
+    hence "D' \<le> C'"
+      using d'_le_d le_trans by blast
     hence max_d': "Max (atms_of D') = A"
       using a_in_d' max_c' by (fast intro: pos_lit_in_atms_of le_multiset_Max_in_imp_Max)
 
@@ -356,14 +356,14 @@ proof -
       hence "Interp D' \<Turnstile> D'"
         using a_in_d' max_d' by (blast intro: max_atm_imp_true_in_Interp)
       hence "Interp D \<Turnstile> D'"
-        using d'_le_d by (auto intro: true_Interp_imp_Interp simp: le_multiset_def)
+        using d'_le_d by (auto intro: true_Interp_imp_Interp simp: less_eq_multiset_def)
       hence False
         using d'_at_d by satx }
     moreover
     { assume "Max (atms_of D') < Max (atms_of D)"
       hence False
         using max_d' leq_dc' max_c' d'_le_d
-        by (metis leD less_eq_Max_atms_of le_multiset_empty_right order.strict_implies_not_eq) }
+        by (metis le_imp_less_or_eq le_multiset_empty_right less_eq_Max_atms_of less_imp_not_less) }
     ultimately have False
       using in_n_or_max_gt by satx }
   thus ?thesis
@@ -371,20 +371,20 @@ proof -
 qed
 
 lemma false_Interp_imp_interp:
-  "D' #\<subseteq># D \<Longrightarrow> D' \<in> N \<and> S D' = {#} \<or> Max (atms_of D') < Max (atms_of D) \<Longrightarrow> \<not> Interp D \<Turnstile> D' \<Longrightarrow>
-   D #\<subset># C \<Longrightarrow> \<not> interp C \<Turnstile> D'"
+  "D' \<le> D \<Longrightarrow> D' \<in> N \<and> S D' = {#} \<or> Max (atms_of D') < Max (atms_of D) \<Longrightarrow> \<not> Interp D \<Turnstile> D' \<Longrightarrow>
+   D < C \<Longrightarrow> \<not> interp C \<Turnstile> D'"
   using interp_def false_Interp_imp_general by simp
 
 lemma false_Interp_imp_Interp:
-  "D' #\<subseteq># D \<Longrightarrow> D' \<in> N \<and> S D' = {#} \<or> Max (atms_of D') < Max (atms_of D) \<Longrightarrow> \<not> Interp D \<Turnstile> D' \<Longrightarrow>
-   D #\<subset># C \<Longrightarrow> \<not> Interp C \<Turnstile> D'"
+  "D' \<le> D \<Longrightarrow> D' \<in> N \<and> S D' = {#} \<or> Max (atms_of D') < Max (atms_of D) \<Longrightarrow> \<not> Interp D \<Turnstile> D' \<Longrightarrow>
+   D < C \<Longrightarrow> \<not> Interp C \<Turnstile> D'"
   using Interp_as_UNION interp_subseteq_Interp false_Interp_imp_general by metis
 
 lemma false_Interp_imp_INTERP:
-  "D' #\<subseteq># D \<Longrightarrow> D' \<in> N \<and> S D' = {#} \<or> Max (atms_of D') < Max (atms_of D) \<Longrightarrow> \<not> Interp D \<Turnstile> D' \<Longrightarrow>
+  "D' \<le> D \<Longrightarrow> D' \<in> N \<and> S D' = {#} \<or> Max (atms_of D') < Max (atms_of D) \<Longrightarrow> \<not> Interp D \<Turnstile> D' \<Longrightarrow>
    \<not> INTERP \<Turnstile> D'"
   using INTERP_def interp_subseteq_INTERP
-    false_Interp_imp_general[OF _ _ _ less_multiset_right_total]
+    false_Interp_imp_general[OF _ _ _ le_multiset_right_total]
   by simp
 
 text {*
@@ -400,13 +400,13 @@ the counterexample).
 *}
 
 lemma
-  assumes "D \<in> N" and "\<And>D'. D' #\<subset># D \<Longrightarrow> Interp D' \<Turnstile> C"
+  assumes "D \<in> N" and "\<And>D'. D' < D \<Longrightarrow> Interp D' \<Turnstile> C"
   shows "interp D \<Turnstile> C"
   oops
 
 lemma
   assumes d: "D = {#}" and n: "N = {D}" and c: "C = {#Pos A#}"
-  shows "D \<in> N" and "\<And>D'. D' #\<subset># D \<Longrightarrow> Interp D' \<Turnstile> C" and "\<not> interp D \<Turnstile> C"
+  shows "D \<in> N" and "\<And>D'. D' < D \<Longrightarrow> Interp D' \<Turnstile> C" and "\<not> interp D \<Turnstile> C"
   using n unfolding d c interp_def by auto
 
 end
