lib/Multiset_More.thy
@@ -114,25 +114,29 @@ lemma size_psubset: "(\<Sigma>:: _ multiset) \<le># \<Sigma>' \<Longrightarrow> 
   using less_irrefl subset_mset_def by blast
 
 
-subsection \<open>Multiset Extension of Multiset Ordering\<close>
+(* subsection \<open>Multiset Extension of Multiset Ordering\<close>
 
 text \<open>
-The \<open>op #\<subset>##\<close> and \<open>op #\<subseteq>##\<close> operators are introduced as the multiset extension of
-the multiset orderings of @{term "op #\<subset>#"} and @{term "op #\<subseteq>#"}.
+The \<open>op <#\<close> and \<open>op \<le>#\<close> operators are introduced as the multiset extension of
+the multiset orderings of @{term "op <"} and @{term "op \<le>"}.
 \<close>
 
 definition less_mset_mset :: "('a :: order) multiset multiset \<Rightarrow> 'a multiset multiset \<Rightarrow> bool"
   (infix "#<##" 50)
 where
-  "M' #<## M \<longleftrightarrow> (M', M) \<in> mult {(x', x). x' #<# x}"
+  "M' #<## M \<longleftrightarrow> (M', M) \<in> mult {(x', x). x' < x}"
 
+lemma
+  fixes M M' :: "'a :: order multiset multiset"
+  shows "M < M' \<longleftrightarrow> M #<## M'"
+  unfolding less_mset_mset_def less_multiset_def ..
 definition le_mset_mset :: "('a :: order) multiset multiset \<Rightarrow> 'a multiset multiset \<Rightarrow> bool"
   (infix "#<=##" 50)
 where
   "M' #<=## M \<longleftrightarrow> M' #<## M \<or> M' = M"
 
-notation less_mset_mset (infix "#\<subset>##" 50)
-notation le_mset_mset (infix "#\<subseteq>##" 50)
+notation less_mset_mset (infix "<#" 50)
+notation le_mset_mset (infix "\<le>#" 50)
 
 lemmas less_mset_mset\<^sub>D\<^sub>M = order.mult\<^sub>D\<^sub>M[OF order_multiset, folded less_mset_mset_def]
 lemmas less_mset_mset\<^sub>H\<^sub>O = order.mult\<^sub>H\<^sub>O[OF order_multiset, folded less_mset_mset_def]
@@ -149,7 +153,7 @@ interpretation multiset_multiset_linorder: linorder
   unfolding less_mset_mset_def[abs_def] le_mset_mset_def[abs_def]
   by (rule linorder.linorder_mult[OF linorder_multiset])
 
-lemma wf_less_mset_mset: "wf {(\<Sigma> :: ('a :: wellorder) multiset multiset, T). \<Sigma> #\<subset>## T}"
+lemma wf_less_mset_mset: "wf {(\<Sigma> :: ('a :: wellorder) multiset multiset, T). \<Sigma> <# T}"
   unfolding less_mset_mset_def by (auto intro: wf_mult wf_less_multiset)
 
 interpretation multiset_multiset_wellorder: wellorder
@@ -157,22 +161,36 @@ interpretation multiset_multiset_wellorder: wellorder
   "less_mset_mset :: ('a::wellorder) multiset multiset \<Rightarrow> ('a::wellorder) multiset multiset \<Rightarrow> bool"
   by unfold_locales (blast intro: wf_less_mset_mset[unfolded wf_def, rule_format])
 
-lemma union_less_mset_mset_mono2: "B #\<subset>## D \<Longrightarrow> C + B #\<subset>## C + (D::'a::order multiset multiset)"
+lemma union_less_mset_mset_mono2: "B <# D \<Longrightarrow> C + B <# C + (D::'a::order multiset multiset)"
 apply (unfold less_mset_mset_def mult_def)
 apply (erule trancl_induct)
  apply (blast intro: mult1_union)
 apply (blast intro: mult1_union trancl_trans)
 done
 
-lemma union_less_mset_mset_diff_plus:
-  "U \<le># \<Sigma> \<Longrightarrow> T #\<subset>## U \<Longrightarrow> \<Sigma> - U + T #\<subset>## \<Sigma>"
-  apply (drule subset_mset.diff_add[symmetric])
-  using union_less_mset_mset_mono2[of T U "\<Sigma> - U"] by simp
+T U "\<Sigma> - U"] by simp
 
 lemma ex_gt_imp_less_mset_mset:
-  "(\<exists>y :: 'a :: linorder multiset \<in># T. (\<forall>x. x \<in># \<Sigma> \<longrightarrow> x #\<subset># y)) \<Longrightarrow> \<Sigma> #\<subset>## T"
+  "(\<exists>y :: 'a :: linorder multiset \<in># T. (\<forall>x. x \<in># \<Sigma> \<longrightarrow> x < y)) \<Longrightarrow> \<Sigma> <# T"
   using less_mset_mset\<^sub>H\<^sub>O by (metis count_greater_zero_iff count_inI less_nat_zero_code
     multiset_linorder.not_less_iff_gr_or_eq)
+ *)
+lemma ex_gt_imp_less_mset_mset:
+  "(\<exists>y :: 'a :: linorder multiset \<in># T. (\<forall>x. x \<in># \<Sigma> \<longrightarrow> x < y)) \<Longrightarrow> \<Sigma> < T"
+  using order.mult\<^sub>H\<^sub>O[OF order_multiset,  folded less_multiset_def] by (metis count_greater_zero_iff count_inI less_nat_zero_code
+    multiset_linorder.not_less_iff_gr_or_eq)
+  
+instantiation multiset :: (linorder) linorder
+begin
+instance
+  by standard (fastforce simp add: less_multiset\<^sub>H\<^sub>O less_eq_multiset_def not_less_iff_gr_or_eq)
+end
+
+instantiation multiset :: (wellorder) wellorder
+begin
+instance
+  by standard (blast intro: wf_less_multiset [unfolded wf_def, simplified, rule_format])
+end
 
 
 subsection \<open>Remove\<close>
@@ -618,28 +636,6 @@ lemma msetsum_union_disjoint:
   shows "(\<Sum>La\<in>#A #\<union> B. f La) = (\<Sum>La\<in>#A. f La) + (\<Sum>La\<in>#B. f La)"
   by (metis assms diff_zero empty_sup image_mset_union msetsum.union multiset_inter_commute
     multiset_union_diff_commute sup_subset_mset_def zero_diff)
-
-
-subsection \<open>Order\<close>
-
-text \<open>Instantiating multiset order as a linear order.
-
-  TODO: remove when multiset is of sort ord again\<close>
-instantiation multiset :: (linorder) linorder
-begin
-
-definition less_multiset :: "'a::linorder multiset \<Rightarrow> 'a multiset \<Rightarrow> bool" where
-  "M' < M \<longleftrightarrow> M' #\<subset># M"
-
-definition less_eq_multiset :: "'a multiset \<Rightarrow> 'a multiset \<Rightarrow>bool" where
-   "(M'::'a multiset) \<le> M \<longleftrightarrow> M' #\<subseteq># M"
-
-instance
-  by standard (auto simp add: less_eq_multiset_def less_multiset_def multiset_order.less_le_not_le
-    add.commute multiset_order.add_right_mono)
-end
-
-
 
 
 section \<open>Cartesian Product\<close>
